latch1 → waiter.

theories/std/mpsc_waiter.v
@@ -29,14 +29,14 @@ Implicit Types l : location.
 )(in custom zebre_field
 ).
 
-Definition mpsc_latch1_create : val :=
+Definition mpsc_waiter_create : val :=
   λ: <>,
     { #false;
       mutex_create ();
       condition_create ()
     }.
 
-Definition mpsc_latch1_signal : val :=
+Definition mpsc_waiter_signal : val :=
   λ: "t",
     if: "t".{flag} then (
       #true
@@ -55,13 +55,13 @@ Definition mpsc_latch1_signal : val :=
       "res"
     ).
 
-Definition mpsc_latch1_try_wait : val :=
+Definition mpsc_waiter_try_wait : val :=
   λ: "t",
     "t".{flag}.
 
-Definition mpsc_latch1_wait : val :=
+Definition mpsc_waiter_wait : val :=
   λ: "t",
-    ifnot: mpsc_latch1_try_wait "t" then (
+    ifnot: mpsc_waiter_try_wait "t" then (
       let: "mtx" := "t".{mutex} in
       let: "cond" := "t".{condition} in
       mutex_protect "mtx" (λ: <>,
@@ -69,58 +69,58 @@ Definition mpsc_latch1_wait : val :=
       )
     ).
 
-Class MpscLatch1G Σ `{zebre_G : !ZebreG Σ} := {
-  #[local] mpsc_latch1_G_mutex_G :: MutexG Σ ;
-  #[local] mpsc_latch1_G_lstate_G :: OneshotG Σ unit unit ;
-  #[local] mpsc_latch1_G_consumer_G :: ExclG Σ unitO ;
+Class MpscWaiterG Σ `{zebre_G : !ZebreG Σ} := {
+  #[local] mpsc_waiter_G_mutex_G :: MutexG Σ ;
+  #[local] mpsc_waiter_G_lstate_G :: OneshotG Σ unit unit ;
+  #[local] mpsc_waiter_G_consumer_G :: ExclG Σ unitO ;
 }.
 
-Definition mpsc_latch1_Σ := #[
+Definition mpsc_waiter_Σ := #[
   mutex_Σ ;
   oneshot_Σ unit unit ;
   excl_Σ unitO
 ].
-#[global] Instance subG_mpsc_latch1_Σ Σ `{zebre_G : !ZebreG Σ} :
-  subG mpsc_latch1_Σ Σ →
-  MpscLatch1G Σ .
+#[global] Instance subG_mpsc_waiter_Σ Σ `{zebre_G : !ZebreG Σ} :
+  subG mpsc_waiter_Σ Σ →
+  MpscWaiterG Σ .
 Proof.
   solve_inG.
 Qed.
 
-Section mpsc_latch1_G.
-  Context `{mpsc_latch1_G : MpscLatch1G Σ}.
+Section mpsc_waiter_G.
+  Context `{mpsc_waiter_G : MpscWaiterG Σ}.
 
-  Record mpsc_latch1_meta := {
-    mpsc_latch1_meta_lstate : gname ;
-    mpsc_latch1_meta_consumer : gname ;
+  Record mpsc_waiter_meta := {
+    mpsc_waiter_meta_lstate : gname ;
+    mpsc_waiter_meta_consumer : gname ;
   }.
-  Implicit Types γ : mpsc_latch1_meta.
+  Implicit Types γ : mpsc_waiter_meta.
 
-  #[local] Instance mpsc_latch1_meta_eq_dec : EqDecision mpsc_latch1_meta :=
+  #[local] Instance mpsc_waiter_meta_eq_dec : EqDecision mpsc_waiter_meta :=
     ltac:(solve_decision).
-  #[local] Instance mpsc_latch1_meta_countable :
-    Countable mpsc_latch1_meta.
+  #[local] Instance mpsc_waiter_meta_countable :
+    Countable mpsc_waiter_meta.
   Proof.
     pose encode γ := (
-      γ.(mpsc_latch1_meta_lstate),
-      γ.(mpsc_latch1_meta_consumer)
+      γ.(mpsc_waiter_meta_lstate),
+      γ.(mpsc_waiter_meta_consumer)
     ).
     pose decode := λ '(γ_lstate, γ_consumer), {|
-      mpsc_latch1_meta_lstate := γ_lstate ;
-      mpsc_latch1_meta_consumer := γ_consumer ;
+      mpsc_waiter_meta_lstate := γ_lstate ;
+      mpsc_waiter_meta_consumer := γ_consumer ;
     |}.
     refine (inj_countable' encode decode _). intros []. done.
   Qed.
 
-  #[local] Definition mpsc_latch1_inv_inner l γ P : iProp Σ :=
+  #[local] Definition mpsc_waiter_inv_inner l γ P : iProp Σ :=
     ∃ b,
     l.[flag] ↦ #b ∗
     if b then
-      oneshot_shot γ.(mpsc_latch1_meta_lstate) () ∗
-      (P ∨ excl γ.(mpsc_latch1_meta_consumer) ())
+      oneshot_shot γ.(mpsc_waiter_meta_lstate) () ∗
+      (P ∨ excl γ.(mpsc_waiter_meta_consumer) ())
     else
-      oneshot_pending γ.(mpsc_latch1_meta_lstate) (DfracOwn 1) ().
-  Definition mpsc_latch1_inv t P : iProp Σ :=
+      oneshot_pending γ.(mpsc_waiter_meta_lstate) (DfracOwn 1) ().
+  Definition mpsc_waiter_inv t P : iProp Σ :=
     ∃ l γ mtx cond,
     ⌜t = #l⌝ ∗
     meta l nroot γ ∗
@@ -128,60 +128,60 @@ Section mpsc_latch1_G.
     mutex_inv mtx True ∗
     l.[condition] ↦□ cond ∗
     condition_inv cond ∗
-    inv nroot (mpsc_latch1_inv_inner l γ P).
+    inv nroot (mpsc_waiter_inv_inner l γ P).
 
-  Definition mpsc_latch1_consumer t : iProp Σ :=
+  Definition mpsc_waiter_consumer t : iProp Σ :=
     ∃ l γ,
     ⌜t = #l⌝ ∗
     meta l nroot γ ∗
-    excl γ.(mpsc_latch1_meta_consumer) ().
+    excl γ.(mpsc_waiter_meta_consumer) ().
 
-  Definition mpsc_latch1_signaled t : iProp Σ :=
+  Definition mpsc_waiter_signaled t : iProp Σ :=
     ∃ l γ,
     ⌜t = #l⌝ ∗
     meta l nroot γ ∗
-    oneshot_shot γ.(mpsc_latch1_meta_lstate) ().
+    oneshot_shot γ.(mpsc_waiter_meta_lstate) ().
 
-  #[global] Instance mpsc_latch1_inv_contractive t :
-    Contractive (mpsc_latch1_inv t).
+  #[global] Instance mpsc_waiter_inv_contractive t :
+    Contractive (mpsc_waiter_inv t).
   Proof.
-    rewrite /mpsc_latch1_inv /mpsc_latch1_inv_inner. solve_contractive.
+    rewrite /mpsc_waiter_inv /mpsc_waiter_inv_inner. solve_contractive.
   Qed.
-  #[global] Instance mpsc_latch1_inv_ne t :
-    NonExpansive (mpsc_latch1_inv t).
-  Proof.
-    apply _.
-  Qed.
-  #[global] Instance mpsc_latch1_inv_proper t :
-    Proper ((≡) ==> (≡)) (mpsc_latch1_inv t).
+  #[global] Instance mpsc_waiter_inv_ne t :
+    NonExpansive (mpsc_waiter_inv t).
   Proof.
     apply _.
   Qed.
-
-  #[global] Instance mpsc_latch1_inv_persistent t P :
-    Persistent (mpsc_latch1_inv t P).
-  Proof.
-    apply _.
-  Qed.
-  #[global] Instance mpsc_latch1_signaled_persistent t :
-    Persistent (mpsc_latch1_signaled t).
-  Proof.
-    apply _.
-  Qed.
-  #[global] Instance mpsc_latch1_consumer_timeless t :
-    Timeless (mpsc_latch1_consumer t).
-  Proof.
-    apply _.
-  Qed.
-  #[global] Instance mpsc_latch1_signaled_timeless t :
-    Timeless (mpsc_latch1_signaled t).
+  #[global] Instance mpsc_waiter_inv_proper t :
+    Proper ((≡) ==> (≡)) (mpsc_waiter_inv t).
   Proof.
     apply _.
   Qed.
 
-  Lemma mpsc_latch1_consumer_exclusive t :
-    mpsc_latch1_consumer t -∗
-    mpsc_latch1_consumer t -∗
+  #[global] Instance mpsc_waiter_inv_persistent t P :
+    Persistent (mpsc_waiter_inv t P).
+  Proof.
+    apply _.
+  Qed.
+  #[global] Instance mpsc_waiter_signaled_persistent t :
+    Persistent (mpsc_waiter_signaled t).
+  Proof.
+    apply _.
+  Qed.
+  #[global] Instance mpsc_waiter_consumer_timeless t :
+    Timeless (mpsc_waiter_consumer t).
+  Proof.
+    apply _.
+  Qed.
+  #[global] Instance mpsc_waiter_signaled_timeless t :
+    Timeless (mpsc_waiter_signaled t).
+  Proof.
+    apply _.
+  Qed.
+
+  Lemma mpsc_waiter_consumer_exclusive t :
+    mpsc_waiter_consumer t -∗
+    mpsc_waiter_consumer t -∗
     False.
   Proof.
     iIntros "(%l & %γ & -> & #Hmeta & Hconsumer1) (%_l & %_γ & %Heq & _Hmeta & Hconsumer2)". injection Heq as <-.
@@ -189,13 +189,13 @@ Section mpsc_latch1_G.
     iApply (excl_exclusive with "Hconsumer1 Hconsumer2").
   Qed.
 
-  Lemma mpsc_latch1_create_spec P :
+  Lemma mpsc_waiter_create_spec P :
     {{{ True }}}
-      mpsc_latch1_create ()
+      mpsc_waiter_create ()
     {{{ t,
       RET t;
-      mpsc_latch1_inv t P ∗
-      mpsc_latch1_consumer t
+      mpsc_waiter_inv t P ∗
+      mpsc_waiter_consumer t
     }}}.
   Proof.
     iIntros "%Φ _ HΦ".
@@ -209,26 +209,26 @@ Section mpsc_latch1_G.
 
     iMod (oneshot_alloc ()) as "(%γ_lstate & Hpending)".
 
-    iMod (excl_alloc (excl_G := mpsc_latch1_G_consumer_G) ()) as "(%γ_consumer & Hconsumer)".
+    iMod (excl_alloc (excl_G := mpsc_waiter_G_consumer_G) ()) as "(%γ_consumer & Hconsumer)".
 
     pose γ := {|
-      mpsc_latch1_meta_lstate := γ_lstate ;
-      mpsc_latch1_meta_consumer := γ_consumer ;
+      mpsc_waiter_meta_lstate := γ_lstate ;
+      mpsc_waiter_meta_consumer := γ_consumer ;
     |}.
     iMod (meta_set _ _ γ with "Hmeta") as "#Hmeta"; first done.
 
     iSteps.
   Qed.
 
-  Lemma mpsc_latch1_signal_spec t P :
+  Lemma mpsc_waiter_signal_spec t P :
     {{{
-      mpsc_latch1_inv t P ∗
+      mpsc_waiter_inv t P ∗
       P
     }}}
-      mpsc_latch1_signal t
+      mpsc_waiter_signal t
     {{{ b,
       RET #b;
-      mpsc_latch1_signaled t
+      mpsc_waiter_signaled t
     }}}.
   Proof.
     iIntros "%Φ ((%l & %γ & %mtx & %cond & -> & #Hmeta & #Hmtx & #Hmtx_inv & #Hcond & #Hcond_inv & #Hinv) & HP) HΦ".
@@ -247,7 +247,7 @@ Section mpsc_latch1_G.
     pose (Ψ_mtx res := (
       ∃ b,
       ⌜res = #b⌝ ∗
-      oneshot_shot γ.(mpsc_latch1_meta_lstate)  ()
+      oneshot_shot γ.(mpsc_waiter_meta_lstate)  ()
     )%I).
     wp_smart_apply (mutex_protect_spec Ψ_mtx with "[$Hmtx_inv HP]"); last first.
     { iSteps. iModIntro.
@@ -274,13 +274,13 @@ Section mpsc_latch1_G.
     iSteps.
   Qed.
 
-  Lemma mpsc_latch1_try_wait_spec_signaled t P :
+  Lemma mpsc_waiter_try_wait_spec_signaled t P :
     {{{
-      mpsc_latch1_inv t P ∗
-      mpsc_latch1_consumer t ∗
-      mpsc_latch1_signaled t
+      mpsc_waiter_inv t P ∗
+      mpsc_waiter_consumer t ∗
+      mpsc_waiter_signaled t
     }}}
-      mpsc_latch1_try_wait t
+      mpsc_waiter_try_wait t
     {{{
       RET #true;
       P
@@ -301,18 +301,18 @@ Section mpsc_latch1_G.
     { iDestruct (excl_exclusive with "Hconsumer Hconsumer'") as %[]. }
     iSmash.
   Qed.
-  Lemma mpsc_latch1_try_wait_spec t P :
+  Lemma mpsc_waiter_try_wait_spec t P :
     {{{
-      mpsc_latch1_inv t P ∗
-      mpsc_latch1_consumer t
+      mpsc_waiter_inv t P ∗
+      mpsc_waiter_consumer t
     }}}
-      mpsc_latch1_try_wait t
+      mpsc_waiter_try_wait t
     {{{ b,
       RET #b;
       if b then
         P
       else
-        mpsc_latch1_consumer t
+        mpsc_waiter_consumer t
     }}}.
   Proof.
     iIntros "%Φ ((%l & %γ & %mtx & %cond & -> & #Hmeta & #Hmtx & #Hmtx_inv & #Hcond & #Hcond_inv & #Hinv) & (%_l & %_γ & %Heq & _Hmeta & Hconsumer)) HΦ". injection Heq as <-.
@@ -329,12 +329,12 @@ Section mpsc_latch1_G.
     iSmash.
   Qed.
 
-  Lemma mpsc_latch1_wait_spec t P :
+  Lemma mpsc_waiter_wait_spec t P :
     {{{
-      mpsc_latch1_inv t P ∗
-      mpsc_latch1_consumer t
+      mpsc_waiter_inv t P ∗
+      mpsc_waiter_consumer t
     }}}
-      mpsc_latch1_wait t
+      mpsc_waiter_wait t
     {{{
       RET ();
       P
@@ -343,7 +343,7 @@ Section mpsc_latch1_G.
     iIntros "%Φ (#Hinv & Hconsumer) HΦ".
 
     wp_rec.
-    wp_apply (mpsc_latch1_try_wait_spec with "[$Hinv $Hconsumer]") as ([]) "Hconsumer"; first iSteps.
+    wp_apply (mpsc_waiter_try_wait_spec with "[$Hinv $Hconsumer]") as ([]) "Hconsumer"; first iSteps.
 
     iDestruct "Hinv" as "(%l & %γ & %mtx & %cond & -> & #Hmeta & #Hmtx & #Hmtx_inv & #Hcond & #Hcond_inv & #Hinv)".
     iDestruct "Hconsumer" as "(%_l & %_γ & %Heq & _Hmeta & Hconsumer)". injection Heq as <-.
@@ -360,7 +360,7 @@ Section mpsc_latch1_G.
       if b then
         P
       else
-        excl γ.(mpsc_latch1_meta_consumer) ()
+        excl γ.(mpsc_waiter_meta_consumer) ()
     )%I).
     wp_smart_apply (condition_wait_until_spec Ψ_cond with "[$Hcond_inv $Hmtx_inv $Hmtx_locked $Hconsumer]"); last iSteps.
 
@@ -374,13 +374,13 @@ Section mpsc_latch1_G.
     { iDestruct (excl_exclusive with "Hconsumer Hconsumer'") as %[]. }
     iSmash.
   Qed.
-End mpsc_latch1_G.
+End mpsc_waiter_G.
 
-#[global] Opaque mpsc_latch1_create.
-#[global] Opaque mpsc_latch1_signal.
-#[global] Opaque mpsc_latch1_try_wait.
-#[global] Opaque mpsc_latch1_wait.
+#[global] Opaque mpsc_waiter_create.
+#[global] Opaque mpsc_waiter_signal.
+#[global] Opaque mpsc_waiter_try_wait.
+#[global] Opaque mpsc_waiter_wait.
 
-#[global] Opaque mpsc_latch1_inv.
-#[global] Opaque mpsc_latch1_consumer.
-#[global] Opaque mpsc_latch1_signaled.
+#[global] Opaque mpsc_waiter_inv.
+#[global] Opaque mpsc_waiter_consumer.
+#[global] Opaque mpsc_waiter_signaled.
