theories/std/spsc_waiter.v
@@ -29,25 +29,25 @@ Implicit Types l : location.
 )(in custom zebre_field
 ).
 
-Definition spsc_latch1_create : val :=
+Definition spsc_waiter_create : val :=
   λ: <>,
     { #false;
       mutex_create ();
       condition_create ()
     }.
 
-Definition spsc_latch1_signal : val :=
+Definition spsc_waiter_signal : val :=
   λ: "t",
     "t" <-{flag} #true ;;
     condition_signal "t".{condition}.
 
-Definition spsc_latch1_try_wait : val :=
+Definition spsc_waiter_try_wait : val :=
   λ: "t",
     "t".{flag}.
 
-Definition spsc_latch1_wait : val :=
+Definition spsc_waiter_wait : val :=
   λ: "t",
-    ifnot: spsc_latch1_try_wait "t" then (
+    ifnot: spsc_waiter_try_wait "t" then (
       let: "mtx" := "t".{mutex} in
       let: "cond" := "t".{condition} in
       mutex_protect "mtx" (λ: <>,
@@ -55,58 +55,58 @@ Definition spsc_latch1_wait : val :=
       )
     ).
 
-Class SpscLatch1G Σ `{zebre_G : !ZebreG Σ} := {
-  #[local] spsc_latch1_G_mutex_G :: MutexG Σ ;
-  #[local] spsc_latch1_G_lstate_G :: OneshotG Σ unit unit ;
-  #[local] spsc_latch1_G_excl_G :: ExclG Σ unitO ;
+Class SpscWaiterG Σ `{zebre_G : !ZebreG Σ} := {
+  #[local] spsc_waiter_G_mutex_G :: MutexG Σ ;
+  #[local] spsc_waiter_G_lstate_G :: OneshotG Σ unit unit ;
+  #[local] spsc_waiter_G_excl_G :: ExclG Σ unitO ;
 }.
 
-Definition spsc_latch1_Σ := #[
+Definition spsc_waiter_Σ := #[
   mutex_Σ ;
   oneshot_Σ unit unit ;
   excl_Σ unitO
 ].
-#[global] Instance subG_spsc_latch1_Σ Σ `{zebre_G : !ZebreG Σ} :
-  subG spsc_latch1_Σ Σ →
-  SpscLatch1G Σ .
+#[global] Instance subG_spsc_waiter_Σ Σ `{zebre_G : !ZebreG Σ} :
+  subG spsc_waiter_Σ Σ →
+  SpscWaiterG Σ .
 Proof.
   solve_inG.
 Qed.
 
-Section spsc_latch1_G.
-  Context `{spsc_latch1_G : SpscLatch1G Σ}.
+Section spsc_waiter_G.
+  Context `{spsc_waiter_G : SpscWaiterG Σ}.
 
-  Record spsc_latch1_meta := {
-    spsc_latch1_meta_lstate : gname ;
-    spsc_latch1_meta_consumer : gname ;
+  Record spsc_waiter_meta := {
+    spsc_waiter_meta_lstate : gname ;
+    spsc_waiter_meta_consumer : gname ;
   }.
-  Implicit Types γ : spsc_latch1_meta.
+  Implicit Types γ : spsc_waiter_meta.
 
-  #[local] Instance spsc_latch1_meta_eq_dec : EqDecision spsc_latch1_meta :=
+  #[local] Instance spsc_waiter_meta_eq_dec : EqDecision spsc_waiter_meta :=
     ltac:(solve_decision).
-  #[local] Instance spsc_latch1_meta_countable :
-    Countable spsc_latch1_meta.
+  #[local] Instance spsc_waiter_meta_countable :
+    Countable spsc_waiter_meta.
   Proof.
     pose encode γ := (
-      γ.(spsc_latch1_meta_lstate),
-      γ.(spsc_latch1_meta_consumer)
+      γ.(spsc_waiter_meta_lstate),
+      γ.(spsc_waiter_meta_consumer)
     ).
     pose decode := λ '(γ_lstate, γ_consumer), {|
-      spsc_latch1_meta_lstate := γ_lstate ;
-      spsc_latch1_meta_consumer := γ_consumer ;
+      spsc_waiter_meta_lstate := γ_lstate ;
+      spsc_waiter_meta_consumer := γ_consumer ;
     |}.
     refine (inj_countable' encode decode _). intros []. done.
   Qed.
 
-  #[local] Definition spsc_latch1_inv_inner l γ P : iProp Σ :=
+  #[local] Definition spsc_waiter_inv_inner l γ P : iProp Σ :=
     ∃ b,
     l.[flag] ↦ #b ∗
     if b then
-      oneshot_shot γ.(spsc_latch1_meta_lstate) () ∗
-      (P ∨ excl γ.(spsc_latch1_meta_consumer) ())
+      oneshot_shot γ.(spsc_waiter_meta_lstate) () ∗
+      (P ∨ excl γ.(spsc_waiter_meta_consumer) ())
     else
-      oneshot_pending γ.(spsc_latch1_meta_lstate) (DfracOwn (1/3)) ().
-  Definition spsc_latch1_inv t P : iProp Σ :=
+      oneshot_pending γ.(spsc_waiter_meta_lstate) (DfracOwn (1/3)) ().
+  Definition spsc_waiter_inv t P : iProp Σ :=
     ∃ l γ mtx cond,
     ⌜t = #l⌝ ∗
     meta l nroot γ ∗
@@ -114,71 +114,71 @@ Section spsc_latch1_G.
     mutex_inv mtx True ∗
     l.[condition] ↦□ cond ∗
     condition_inv cond ∗
-    inv nroot (spsc_latch1_inv_inner l γ P).
+    inv nroot (spsc_waiter_inv_inner l γ P).
 
-  Definition spsc_latch1_producer t : iProp Σ :=
+  Definition spsc_waiter_producer t : iProp Σ :=
     ∃ l γ,
     ⌜t = #l⌝ ∗
     meta l nroot γ ∗
-    oneshot_pending γ.(spsc_latch1_meta_lstate) (DfracOwn (2/3)) ().
+    oneshot_pending γ.(spsc_waiter_meta_lstate) (DfracOwn (2/3)) ().
 
-  Definition spsc_latch1_consumer t : iProp Σ :=
+  Definition spsc_waiter_consumer t : iProp Σ :=
     ∃ l γ,
     ⌜t = #l⌝ ∗
     meta l nroot γ ∗
-    excl γ.(spsc_latch1_meta_consumer) ().
+    excl γ.(spsc_waiter_meta_consumer) ().
 
-  Definition spsc_latch1_signaled t : iProp Σ :=
+  Definition spsc_waiter_signaled t : iProp Σ :=
     ∃ l γ,
     ⌜t = #l⌝ ∗
     meta l nroot γ ∗
-    oneshot_shot γ.(spsc_latch1_meta_lstate) ().
+    oneshot_shot γ.(spsc_waiter_meta_lstate) ().
 
-  #[global] Instance spsc_latch1_inv_contractive t :
-    Contractive (spsc_latch1_inv t).
+  #[global] Instance spsc_waiter_inv_contractive t :
+    Contractive (spsc_waiter_inv t).
   Proof.
-    rewrite /spsc_latch1_inv /spsc_latch1_inv_inner. solve_contractive.
+    rewrite /spsc_waiter_inv /spsc_waiter_inv_inner. solve_contractive.
   Qed.
-  #[global] Instance spsc_latch1_inv_ne t :
-    NonExpansive (spsc_latch1_inv t).
-  Proof.
-    apply _.
-  Qed.
-  #[global] Instance spsc_latch1_inv_proper t :
-    Proper ((≡) ==> (≡)) (spsc_latch1_inv t).
+  #[global] Instance spsc_waiter_inv_ne t :
+    NonExpansive (spsc_waiter_inv t).
   Proof.
     apply _.
   Qed.
-
-  #[global] Instance spsc_latch1_inv_persistent t P :
-    Persistent (spsc_latch1_inv t P).
-  Proof.
-    apply _.
-  Qed.
-  #[global] Instance spsc_latch1_signaled_persistent t :
-    Persistent (spsc_latch1_signaled t).
-  Proof.
-    apply _.
-  Qed.
-  #[global] Instance spsc_latch1_producer_timeless t :
-    Timeless (spsc_latch1_producer t).
-  Proof.
-    apply _.
-  Qed.
-  #[global] Instance spsc_latch1_consumer_timeless t :
-    Timeless (spsc_latch1_consumer t).
-  Proof.
-    apply _.
-  Qed.
-  #[global] Instance spsc_latch1_signaled_timeless t :
-    Timeless (spsc_latch1_signaled t).
+  #[global] Instance spsc_waiter_inv_proper t :
+    Proper ((≡) ==> (≡)) (spsc_waiter_inv t).
   Proof.
     apply _.
   Qed.
 
-  Lemma spsc_latch1_producer_exclusive t :
-    spsc_latch1_producer t -∗
-    spsc_latch1_producer t -∗
+  #[global] Instance spsc_waiter_inv_persistent t P :
+    Persistent (spsc_waiter_inv t P).
+  Proof.
+    apply _.
+  Qed.
+  #[global] Instance spsc_waiter_signaled_persistent t :
+    Persistent (spsc_waiter_signaled t).
+  Proof.
+    apply _.
+  Qed.
+  #[global] Instance spsc_waiter_producer_timeless t :
+    Timeless (spsc_waiter_producer t).
+  Proof.
+    apply _.
+  Qed.
+  #[global] Instance spsc_waiter_consumer_timeless t :
+    Timeless (spsc_waiter_consumer t).
+  Proof.
+    apply _.
+  Qed.
+  #[global] Instance spsc_waiter_signaled_timeless t :
+    Timeless (spsc_waiter_signaled t).
+  Proof.
+    apply _.
+  Qed.
+
+  Lemma spsc_waiter_producer_exclusive t :
+    spsc_waiter_producer t -∗
+    spsc_waiter_producer t -∗
     False.
   Proof.
     iIntros "(%l & %γ & -> & #Hmeta & Hpending1) (%_l & %_γ & %Heq & _Hmeta & Hpending2)". injection Heq as <-.
@@ -186,9 +186,9 @@ Section spsc_latch1_G.
     iDestruct (oneshot_pending_valid_2 with "Hpending1 Hpending2") as %(? & _). done.
   Qed.
 
-  Lemma spsc_latch1_consumer_exclusive t :
-    spsc_latch1_consumer t -∗
-    spsc_latch1_consumer t -∗
+  Lemma spsc_waiter_consumer_exclusive t :
+    spsc_waiter_consumer t -∗
+    spsc_waiter_consumer t -∗
     False.
   Proof.
     iIntros "(%l & %γ & -> & #Hmeta & Hconsumer1) (%_l & %_γ & %Heq & _Hmeta & Hconsumer2)". injection Heq as <-.
@@ -196,14 +196,14 @@ Section spsc_latch1_G.
     iApply (excl_exclusive with "Hconsumer1 Hconsumer2").
   Qed.
 
-  Lemma spsc_latch1_create_spec P :
+  Lemma spsc_waiter_create_spec P :
     {{{ True }}}
-      spsc_latch1_create ()
+      spsc_waiter_create ()
     {{{ t,
       RET t;
-      spsc_latch1_inv t P ∗
-      spsc_latch1_producer t ∗
-      spsc_latch1_consumer t
+      spsc_waiter_inv t P ∗
+      spsc_waiter_producer t ∗
+      spsc_waiter_consumer t
     }}}.
   Proof.
     iIntros "%Φ _ HΦ".
@@ -219,27 +219,27 @@ Section spsc_latch1_G.
     iEval (assert (1 = 2/3 + 1/3)%Qp as -> by compute_done) in "Hpending".
     iDestruct "Hpending" as "(Hpending1 & Hpending2)".
 
-    iMod (excl_alloc (excl_G := spsc_latch1_G_excl_G) ()) as "(%γ_consumer & Hconsumer)".
+    iMod (excl_alloc (excl_G := spsc_waiter_G_excl_G) ()) as "(%γ_consumer & Hconsumer)".
 
     pose γ := {|
-      spsc_latch1_meta_lstate := γ_lstate ;
-      spsc_latch1_meta_consumer := γ_consumer ;
+      spsc_waiter_meta_lstate := γ_lstate ;
+      spsc_waiter_meta_consumer := γ_consumer ;
     |}.
     iMod (meta_set _ _ γ with "Hmeta") as "#Hmeta"; first done.
 
     iSteps.
   Qed.
 
-  Lemma spsc_latch1_signal_spec t P :
+  Lemma spsc_waiter_signal_spec t P :
     {{{
-      spsc_latch1_inv t P ∗
-      spsc_latch1_producer t ∗
+      spsc_waiter_inv t P ∗
+      spsc_waiter_producer t ∗
       P
     }}}
-      spsc_latch1_signal t
+      spsc_waiter_signal t
     {{{
       RET ();
-      spsc_latch1_signaled t
+      spsc_waiter_signaled t
     }}}.
   Proof.
     iIntros "%Φ ((%l & %γ & %mtx & %cond & -> & #Hmeta & #Hmtx & #Hmtx_inv & #Hcond & #Hcond_inv & #Hinv) & (%_l & %_γ & %Heq & _Hmeta & Hpending) & HP) HΦ". injection Heq as <-.
@@ -266,13 +266,13 @@ Section spsc_latch1_G.
     iSteps.
   Qed.
 
-  Lemma spsc_latch1_try_wait_spec_signaled t P :
+  Lemma spsc_waiter_try_wait_spec_signaled t P :
     {{{
-      spsc_latch1_inv t P ∗
-      spsc_latch1_consumer t ∗
-      spsc_latch1_signaled t
+      spsc_waiter_inv t P ∗
+      spsc_waiter_consumer t ∗
+      spsc_waiter_signaled t
     }}}
-      spsc_latch1_try_wait t
+      spsc_waiter_try_wait t
     {{{
       RET #true;
       P
@@ -293,18 +293,18 @@ Section spsc_latch1_G.
     { iDestruct (excl_exclusive with "Hconsumer Hconsumer'") as %[]. }
     iSmash.
   Qed.
-  Lemma spsc_latch1_try_wait_spec t P :
+  Lemma spsc_waiter_try_wait_spec t P :
     {{{
-      spsc_latch1_inv t P ∗
-      spsc_latch1_consumer t
+      spsc_waiter_inv t P ∗
+      spsc_waiter_consumer t
     }}}
-      spsc_latch1_try_wait t
+      spsc_waiter_try_wait t
     {{{ b,
       RET #b;
       if b then
         P
       else
-        spsc_latch1_consumer t
+        spsc_waiter_consumer t
     }}}.
   Proof.
     iIntros "%Φ ((%l & %γ & %mtx & %cond & -> & #Hmeta & #Hmtx & #Hmtx_inv & #Hcond & #Hcond_inv & #Hinv) & (%_l & %_γ & %Heq & _Hmeta & Hconsumer)) HΦ". injection Heq as <-.
@@ -321,12 +321,12 @@ Section spsc_latch1_G.
     iSmash.
   Qed.
 
-  Lemma spsc_latch1_wait_spec t P :
+  Lemma spsc_waiter_wait_spec t P :
     {{{
-      spsc_latch1_inv t P ∗
-      spsc_latch1_consumer t
+      spsc_waiter_inv t P ∗
+      spsc_waiter_consumer t
     }}}
-      spsc_latch1_wait t
+      spsc_waiter_wait t
     {{{
       RET ();
       P
@@ -335,7 +335,7 @@ Section spsc_latch1_G.
     iIntros "%Φ (#Hinv & Hconsumer) HΦ".
 
     wp_rec.
-    wp_apply (spsc_latch1_try_wait_spec with "[$Hinv $Hconsumer]") as ([]) "Hconsumer"; first iSteps.
+    wp_apply (spsc_waiter_try_wait_spec with "[$Hinv $Hconsumer]") as ([]) "Hconsumer"; first iSteps.
 
     iDestruct "Hinv" as "(%l & %γ & %mtx & %cond & -> & #Hmeta & #Hmtx & #Hmtx_inv & #Hcond & #Hcond_inv & #Hinv)".
     iDestruct "Hconsumer" as "(%_l & %_γ & %Heq & _Hmeta & Hconsumer)". injection Heq as <-.
@@ -352,7 +352,7 @@ Section spsc_latch1_G.
       if b then
         P
       else
-        excl γ.(spsc_latch1_meta_consumer) ()
+        excl γ.(spsc_waiter_meta_consumer) ()
     )%I).
     wp_smart_apply (condition_wait_until_spec Ψ_cond with "[$Hcond_inv $Hmtx_inv $Hmtx_locked $Hconsumer]"); last iSteps.
 
@@ -366,14 +366,14 @@ Section spsc_latch1_G.
     { iDestruct (excl_exclusive with "Hconsumer Hconsumer'") as %[]. }
     iSmash.
   Qed.
-End spsc_latch1_G.
+End spsc_waiter_G.
 
-#[global] Opaque spsc_latch1_create.
-#[global] Opaque spsc_latch1_signal.
-#[global] Opaque spsc_latch1_try_wait.
-#[global] Opaque spsc_latch1_wait.
+#[global] Opaque spsc_waiter_create.
+#[global] Opaque spsc_waiter_signal.
+#[global] Opaque spsc_waiter_try_wait.
+#[global] Opaque spsc_waiter_wait.
 
-#[global] Opaque spsc_latch1_inv.
-#[global] Opaque spsc_latch1_producer.
-#[global] Opaque spsc_latch1_consumer.
-#[global] Opaque spsc_latch1_signaled.
+#[global] Opaque spsc_waiter_inv.
+#[global] Opaque spsc_waiter_producer.
+#[global] Opaque spsc_waiter_consumer.
+#[global] Opaque spsc_waiter_signaled.
